code refactorization: renamed lemmas, functions, methods and removed unnecessary predicates

Licenta.dfy
@@ -1,411 +1,739 @@
-datatype Problem = Problem(numberOfObjects: int, knapsackCapacity: int, gains: seq<int>, weights: seq<int>)
+datatype Problem = Problem(n: int, c: int, gains: seq<int>, weights: seq<int>)
 
-predicate hasPositiveValues(input: seq<int>)
+type Solution = seq<int> 
+
+function gain(p: Problem, solution: Solution): int
+  requires isValidProblem(p)
+  requires hasAllowedValues(solution)
+  requires 0 <= |solution| <= p.n
 {
-    forall i :: 0 <= i < |input| ==> input[i] > 0
+  if |solution| == 0 then 0 else computeGain(p.gains, solution, |solution| - 1)
 }
 
-predicate hasOnlyPermittedValues(solution: seq<int>)
+function computeGain(gains: seq<int>, solution: Solution, i: int) : int
+  requires 0 <= i < |solution|
+  requires 0 <= i < |gains|
+  requires hasAllowedValues(solution)
+  requires 0 <= |solution| <= |gains|
+{
+  if i == 0 then solution[0] * gains[0] else solution[i] * gains[i] + computeGain(gains, solution, i - 1)
+}
+
+function computeGainNew(p: Problem, solution: Solution, i: int) : int //try to remove it
+  requires isValidProblem(p)
+  requires 0 <= i < |solution|
+  requires 0 <= i < |p.gains|
+  requires hasAllowedValues(solution)
+  requires 0 <= |solution| <= |p.gains|
+
+  ensures computeGainNew(p, solution, i) == computeGain(p.gains, solution, i)
+  ensures computeGainNew(p, solution, i) >= 0
+{
+  if i == 0 then solution[0] * p.gains[0] else solution[i] * p.gains[i] + computeGainNew(p, solution, i - 1)
+}
+
+function weight(p: Problem, solution: Solution): int
+  requires isValidProblem(p)
+  requires hasAllowedValues(solution)
+  requires 0 <= |solution| <= p.n
+{
+  if |solution| == 0 then 0 else computeWeight(p.weights, solution, |solution| - 1)
+}
+
+function computeWeight(weights: seq<int>, solution: Solution, i: int) : int
+ requires forall i :: 0 <= i < |weights| ==> weights[i] > 0 
+  requires 0 <= i < |solution|
+  requires 0 <= i < |weights|
+  requires hasAllowedValues(solution)
+  requires 0 <= |solution| <= |weights|
+  
+  ensures computeWeight(weights, solution, i) >= 0
+{
+  if i == 0 then solution[0] * weights[0] else solution[i] * weights[i] + computeWeight(weights, solution, i - 1)
+}
+
+function SumAllGains(p: Problem, i: int) : int
+ requires isValidProblem(p)
+ requires 1 <= i <= p.n
+
+ ensures SumAllGains(p, i) >= 0
+{
+  if (i == 1) then p.gains[0] else p.gains[i - 1] + SumAllGains(p, i -1)
+}
+
+predicate hasPositiveValues(solution: Solution)
+{
+  forall i :: 0 <= i < |solution| ==> solution[i] > 0
+}
+
+predicate hasAllowedValues(solution: Solution)
 {
   forall k :: 0 <= k < |solution| ==> solution[k] == 0 || solution[k] == 1
 }
 
 predicate isValidProblem(p: Problem)
 {
-    |p.gains| == |p.weights| == p.numberOfObjects && 
-    p.numberOfObjects > 0 && p.knapsackCapacity >= 0 && 
-    hasPositiveValues(p.gains) && hasPositiveValues(p.weights) 
+  |p.gains| == |p.weights| == p.n && 
+  p.n > 0 && p.c >= 0 && 
+  hasPositiveValues(p.gains) && hasPositiveValues(p.weights) 
 }
 
-function gain(p: Problem, solution: seq<int>): int
-  requires isValidProblem(p)
-  requires hasOnlyPermittedValues(solution)
-  requires 0 <= |solution| <= p.numberOfObjects
 
-  ensures gain(p, solution) == if |solution| == 0 then 0 else computeGain(p.gains, solution, |solution| - 1)
-{
-  if |solution| == 0 then 0 else computeGain(p.gains, solution, |solution| - 1)
-}
-
-function computeGain(gains: seq<int>, solution: seq<int>, i: int) : int
-  requires 0 <= i < |solution|
-  requires 0 <= i < |gains|
-  requires hasOnlyPermittedValues(solution)
-  requires 0 <= |solution| <= |gains|
-
-  ensures computeGain(gains, solution, i) == if i == 0 then solution[0] * gains[0] else solution[i] * gains[i] + computeGain(gains, solution, i - 1)
-{
-  if i == 0 then solution[0] * gains[0] else solution[i] * gains[i] + computeGain(gains, solution, i - 1)
-}
-
-function computeGainNew(p: Problem , solution: seq<int>, i: int) : int
-  requires isValidProblem(p)
-  requires 0 <= i < |solution|
-  requires 0 <= i < |p.gains|
-  requires hasOnlyPermittedValues(solution)
-  requires 0 <= |solution| <= |p.gains|
-  
-  ensures computeGainNew(p, solution, i) == if i == 0 then solution[0] * p.gains[0] else solution[i] * p.gains[i] + computeGainNew(p, solution, i - 1)
-  ensures computeGainNew(p, solution, i) == computeGain(p.gains, solution, i)
-  ensures computeGainNew(p, solution, i) >= 0
-{
-   if i == 0 then solution[0] * p.gains[0] else solution[i] * p.gains[i] + computeGainNew(p, solution, i - 1)
-}
-
-function weight(p: Problem, solution: seq<int>): int
-  requires isValidProblem(p)
-  requires hasOnlyPermittedValues(solution)
-  requires 0 <= |solution| <= p.numberOfObjects
-  
-  ensures weight(p, solution) == if |solution| == 0 then 0 else computeWeight(p.weights, solution, |solution| - 1)
-{
-  if |solution| == 0 then 0 else computeWeight(p.weights, solution, |solution| - 1)
-}
-
-function computeWeight(weights: seq<int>, solution: seq<int>, i: int) : int
- requires forall i :: 0 <= i < |weights| ==> weights[i] > 0 
-  requires 0 <= i < |solution|
-  requires 0 <= i < |weights|
-  requires hasOnlyPermittedValues(solution)
-  requires 0 <= |solution| <= |weights|
-  
-  ensures computeWeight(weights, solution, i) == if i == 0 then solution[0] * weights[0] else solution[i] * weights[i] + computeWeight(weights, solution, i - 1)
-  ensures computeWeight(weights, solution, i) >= 0
-{
-   if i == 0 then solution[0] * weights[0] else solution[i] * weights[i] + computeWeight(weights, solution, i - 1)
-}
-
-predicate isValidPartialSolution(p: Problem, solution: seq<int>)
+predicate isValidPartialSolution(p: Problem, solution: Solution)
   requires isValidProblem(p)
 {
-  hasOnlyPermittedValues(solution)
+  hasAllowedValues(solution) && |solution| <= p.n
 }
 
-predicate isPartialSolutionOfFirstIObjectsAndWeightJ(p: Problem, solution: seq<int>, i: int, j: int)
+predicate isPartialSolution(p: Problem, solution: Solution, i: int, j: int)
   requires isValidProblem(p)
-  requires 0 <= i <= p.numberOfObjects
-  requires 0 <= j <= p.knapsackCapacity
+  requires 0 <= i <= p.n
+  requires 0 <= j <= p.c
 {
   isValidPartialSolution(p, solution) && |solution| == i &&
   weight(p, solution) <= j
 }
 
-predicate isPartialSolution(p: Problem, solution: seq<int>)
-  requires isValidProblem(p)
-{ 
-  isPartialSolutionOfFirstIObjectsAndWeightJ(p, solution, p.numberOfObjects, p.knapsackCapacity)
-}
-
-predicate isSolution(p: Problem, solution: seq<int>)
+predicate isSolution(p: Problem, solution: Solution)
   requires isValidProblem(p)
 {
-  isValidPartialSolution(p, solution) && |solution| == p.numberOfObjects &&
-  weight(p, solution) <= p.knapsackCapacity
+  isValidPartialSolution(p, solution) && |solution| == p.n &&
+  weight(p, solution) <= p.c
 }
 
-ghost predicate isOptimalPartialSolutionOfFirstIObjectsAndWeightJ(p: Problem, solution: seq<int>, i: int, j: int)
+ghost predicate isOptimalPartialSolution(p: Problem, solution: Solution, i: int, j: int)
   requires isValidProblem(p)
-  requires 0 <= i <= p.numberOfObjects
-  requires 0 <= j <= p.knapsackCapacity
+  requires 0 <= i <= p.n
+  requires 0 <= j <= p.c
 {
-  isPartialSolutionOfFirstIObjectsAndWeightJ(p, solution, i, j) &&
-  forall s: seq<int> :: (isPartialSolutionOfFirstIObjectsAndWeightJ(p, s, i, j) && |s| == |solution| ==> gain(p, solution) >= gain(p, s))
+  isPartialSolution(p, solution, i, j) &&
+  forall s: Solution :: (isPartialSolution(p, s, i, j) && |s| == |solution| ==> gain(p, solution) >= gain(p, s))
 }
 
-ghost predicate isOptimalPartialSolution(p: Problem, solution: seq<int>)
-  requires isValidProblem(p)
-{
-    isOptimalPartialSolutionOfFirstIObjectsAndWeightJ(p, solution, p.numberOfObjects, p.knapsackCapacity)
-}
-
-ghost predicate isOptimalSolution(p: Problem, solution: seq<int>)
+ghost predicate isOptimalSolution(p: Problem, solution: Solution)
   requires isValidProblem(p)
   requires isValidPartialSolution(p, solution)
 {
-    isOptimalPartialSolution(p, solution) &&
-    forall s: seq<int> :: (((isOptimalPartialSolution(p, s)) ==> 
-    gain(p, solution) >= gain(p, s)))
+  isOptimalPartialSolution(p, solution, p.n, p.c) &&
+  forall s: Solution :: (((isOptimalPartialSolution(p, s, p.n, p.c)) ==> 
+  gain(p, solution) >= gain(p, s)))
 }
 
-lemma AddingObjectDoesNotExceedsCapacity(p: Problem, i: int, j: int, sol: seq<int>)  
+lemma ComputeWeightFits1(p: Problem, solution: Solution, i: int, j: int)
   requires isValidProblem(p)
-  requires 0 <= |sol| < p.numberOfObjects
+  requires 0 <= |solution| < p.n
   requires 0 <= i < |p.weights|
-  requires hasOnlyPermittedValues(sol)
-  requires 0 <= j <= p.knapsackCapacity + 1
-  requires weight(p, sol) <= j - p.weights[i]
-  requires i == |sol|
+  requires hasAllowedValues(solution)
+  requires 0 <= j <= p.c + 1
+  requires weight(p, solution) <= j - p.weights[i]
+  requires i == |solution|
   
-  ensures computeWeight(p.weights, sol + [1], |sol + [1]| - 1) <= j
+  ensures computeWeight(p.weights, solution + [1], |solution + [1]| - 1) <= j
 {
-  var newSol := sol + [1];
-  assert sol == newSol[..|newSol| - 1];
+  var s' := solution + [1];
+  assert solution == s'[..|s'| - 1];
 
-  for a := 0 to |newSol[..|newSol| - 1]|
-    invariant 0 <= a <= |newSol[..|newSol| - 1]| + 1
-    invariant forall k :: 0 <= k < a ==> computeWeight(p.weights, sol, k) == computeWeight(p.weights, newSol, k)
+  for a := 0 to |s'[..|s'| - 1]|
+    invariant 0 <= a <= |s'[..|s'| - 1]| + 1
+    invariant forall k :: 0 <= k < a ==> computeWeight(p.weights, solution, k) == computeWeight(p.weights, s', k)
   {
-    assert computeWeight(p.weights, sol, a) == computeWeight(p.weights, newSol, a);
+    assert computeWeight(p.weights, solution, a) == computeWeight(p.weights, s', a);
   }
 }
 
-lemma NotAddingObjectDoesNotChangeSolWeight(p: Problem, j: int, sol: seq<int>)
+lemma ComputeWeightFits0(p: Problem, solution: Solution, j: int)
   requires isValidProblem(p)
-  requires hasOnlyPermittedValues(sol)
-  requires 0 <= |sol| < p.numberOfObjects
-  requires weight(p, sol) <= j
+  requires hasAllowedValues(solution)
+  requires 0 <= |solution| < p.n
+  requires weight(p, solution) <= j
   
-  ensures computeWeight(p.weights, sol + [0], |sol + [0]| - 1) <= j 
+  ensures computeWeight(p.weights, solution + [0], |solution + [0]| - 1) <= j 
 {  
-  if |sol| == 0 {
-    assert weight(p, sol) <= j;
+  if |solution| == 0 {
+    assert weight(p, solution) <= j;
   } else {
-    var newSol := sol + [0];
-    assert newSol[..|newSol| - 1] == sol;
-    LastElementIs0ForComputeWeightHelper(p, newSol, |newSol| - 2);
-    assert computeWeight(p.weights, sol + [0], |sol + [0]| - 1) <= j;
+    var s' := solution + [0];
+    assert s'[..|s'| - 1] == solution;
+    ComputeWeightAdd0(p, s', |s'| - 2);
+    assert computeWeight(p.weights, solution + [0], |solution + [0]| - 1) <= j;
   }
 }
 
-lemma LastElementIs0ForComputeWeightHelper(p: Problem, sol: seq<int>, i: int)
+lemma ComputeWeightAdd0(p: Problem, solution: Solution, i: int)
   requires isValidProblem(p)
-  requires hasOnlyPermittedValues(sol)
-  requires 0 <= i < |sol| - 1
+  requires hasAllowedValues(solution)
+  requires 0 <= i < |solution| - 1
   requires 0 <= i < |p.weights|
-  requires 0 <= |sol| <= |p.weights|
-  requires sol[|sol| - 1] == 0
+  requires 0 <= |solution| <= |p.weights|
+  requires solution[|solution| - 1] == 0
   
-  ensures computeWeight(p.weights, sol, i) == computeWeight(p.weights, sol[..|sol| - 1], i)
+  ensures computeWeight(p.weights, solution, i) == computeWeight(p.weights, solution[..|solution| - 1], i)
 { }
 
-lemma LastElementIs0ForWeightHelper(p: Problem, sol: seq<int>)
+lemma WeightAdd0(p: Problem, solution: Solution)
   requires isValidProblem(p)
-  requires hasOnlyPermittedValues(sol)
-  requires 0 < |sol| <= p.numberOfObjects
-  requires sol[|sol| - 1] == 0
+  requires hasAllowedValues(solution)
+  requires 0 < |solution| <= p.n
+  requires solution[|solution| - 1] == 0
   
-  ensures weight(p, sol) == weight(p, sol[..|sol| - 1])
+  ensures weight(p, solution) == weight(p, solution[..|solution| - 1])
 {
-  if |sol| == 1 {
+  if |solution| == 1 {
 
   } else {
-    assert computeWeight(p.weights, sol, |sol| - 1) == computeWeight(p.weights, sol, |sol| - 2);
-    LastElementIs0ForComputeWeightHelper(p, sol, |sol| - 2);
+    assert computeWeight(p.weights, solution, |solution| - 1) == computeWeight(p.weights, solution, |solution| - 2);
+    ComputeWeightAdd0(p, solution, |solution| - 2);
   }
  }
 
-lemma LastElementIs0ForComputeGainHelper(p: Problem, sol: seq<int>, i: int)
+lemma ComputeGainAdd0(p: Problem, solution: Solution, i: int)
   requires isValidProblem(p)
-  requires hasOnlyPermittedValues(sol)
-  requires 0 <= i < |sol| - 1
+  requires hasAllowedValues(solution)
+  requires 0 <= i < |solution| - 1
   requires 0 <= i < |p.gains|
-  requires 0 <= |sol| <= |p.gains|
-  requires sol[|sol| - 1] == 0
+  requires 0 <= |solution| <= |p.gains|
+  requires solution[|solution| - 1] == 0
   
-  ensures computeGain(p.gains, sol, i) == computeGain(p.gains, sol[..|sol| - 1], i)
+  ensures computeGain(p.gains, solution, i) == computeGain(p.gains, solution[..|solution| - 1], i)
 { }
 
-lemma LastElementIs0ForGainHelper(p: Problem, sol: seq<int>)
+lemma GainAdd0(p: Problem, solution: Solution)
   requires isValidProblem(p)
-  requires hasOnlyPermittedValues(sol)
-  requires 0 < |sol| <= p.numberOfObjects
-  requires sol[|sol| - 1] == 0
+  requires hasAllowedValues(solution)
+  requires 0 < |solution| <= p.n
+  requires solution[|solution| - 1] == 0
   
-  ensures gain(p, sol) == gain(p, sol[..|sol| - 1])
+  ensures gain(p, solution) == gain(p, solution[..|solution| - 1])
 { 
-  if |sol| == 1 {
+  if |solution| == 1 {
 
   } else {
-    assert computeGain(p.gains, sol, |sol| - 1) == computeGain(p.gains, sol, |sol| - 2);
-    LastElementIs0ForComputeGainHelper(p, sol, |sol| - 2);
+    assert computeGain(p.gains, solution, |solution| - 1) == computeGain(p.gains, solution, |solution| - 2);
+    ComputeGainAdd0(p, solution, |solution| - 2);
   }
 }
 
-lemma ComputeGainHelper(p: Problem, sol: seq<int>, i: int) 
+lemma ComputeGainRemoveLast(p: Problem, solution: Solution, i: int)
   requires isValidProblem(p)
-  requires hasOnlyPermittedValues(sol)
-  requires 0 <= i < |sol| <= |p.gains|
-  requires sol == sol[..|sol| - 1] + [sol[|sol| - 1]] 
-  requires i <= |sol[..|sol| - 1]| - 1
+  requires hasAllowedValues(solution)
+  requires 0 <= i < |solution| <= |p.gains|
+  requires i <= |solution[..|solution| - 1]| - 1
 
-  ensures computeGain(p.gains, sol, i) == computeGain(p.gains, sol[..|sol| - 1], i)
+  ensures computeGain(p.gains, solution, i) == computeGain(p.gains, solution[..|solution| - 1], i)
+{ 
+  assert solution == solution[..|solution| - 1] + [solution[|solution| - 1]];
+}
+
+lemma GainAdd1(p: Problem, solution: Solution)
+  requires isValidProblem(p)
+  requires hasAllowedValues(solution)
+  requires 0 < |solution| <= p.n
+  requires solution[|solution| - 1] == 1
+
+  ensures gain(p, solution) == gain(p, solution[..|solution| - 1]) + p.gains[|solution| - 1]
+{ 
+   if |solution| == 1 {
+
+  } else {
+    ComputeGainRemoveLast(p, solution, |solution[..|solution| - 1]| - 1);
+    assert computeGain(p.gains, solution, |solution[..|solution| - 1]| - 1) == 
+           computeGain(p.gains, solution[..|solution| - 1], |solution[..|solution| - 1]| - 1);
+  }
+}
+
+lemma ComputeWeightRemoveLast(p: Problem, solution: Solution, i: int)
+  requires isValidProblem(p)
+  requires hasAllowedValues(solution)
+  requires 0 <= i < |solution| <= |p.gains|
+  requires solution == solution[..|solution| - 1] + [solution[|solution| - 1]] 
+  requires i <= |solution[..|solution| - 1]| - 1
+
+  ensures computeWeight(p.weights, solution, i) == computeWeight(p.weights, solution[..|solution| - 1], i)
 { }
 
-lemma LastElementIs1ForGainHelper(p: Problem, sol: seq<int>)
+lemma WeightAdd1(p: Problem, solution: Solution)
   requires isValidProblem(p)
-  requires hasOnlyPermittedValues(sol)
-  requires 0 < |sol| <= p.numberOfObjects
-  requires sol[|sol| - 1] == 1
+  requires hasAllowedValues(solution)
+  requires 0 < |solution| <= p.n
+  requires solution[|solution| - 1] == 1
 
-  ensures gain(p, sol) == gain(p, sol[..|sol| - 1]) + p.gains[|sol| - 1]
+  ensures weight(p, solution) == weight(p, solution[..|solution| - 1]) + p.weights[|solution| - 1]
 { 
-   if |sol| == 1 {
+  if |solution| == 1 {
 
   } else {
-    ComputeGainHelper(p, sol, |sol[..|sol| - 1]| - 1);
-    assert computeGain(p.gains, sol, |sol[..|sol| - 1]| - 1) == computeGain(p.gains, sol[..|sol| - 1], |sol[..|sol| - 1]| - 1);
+    ComputeWeightRemoveLast(p, solution, |solution[..|solution| - 1]| - 1);
+    assert computeWeight(p.weights, solution, |solution[..|solution| - 1]| - 1) == 
+           computeWeight(p.weights, solution[..|solution| - 1], |solution[..|solution| - 1]| - 1);
   }
 }
 
-lemma ComputeWeightHelper(p: Problem, sol: seq<int>, i: int) 
-  requires isValidProblem(p)
-  requires hasOnlyPermittedValues(sol)
-  requires 0 <= i < |sol| <= |p.gains|
-  requires sol == sol[..|sol| - 1] + [sol[|sol| - 1]] 
-  requires i <= |sol[..|sol| - 1]| - 1
-
-  ensures computeWeight(p.weights, sol, i) == computeWeight(p.weights, sol[..|sol| - 1], i)
-{ }
-
-lemma LastElementIs1ForWeightHelper(p: Problem, sol: seq<int>)
-  requires isValidProblem(p)
-  requires hasOnlyPermittedValues(sol)
-  requires 0 < |sol| <= p.numberOfObjects
-  requires sol[|sol| - 1] == 1
-
-  ensures weight(p, sol) == weight(p, sol[..|sol| - 1]) + p.weights[|sol| - 1]
-{ 
-  if |sol| == 1 {
-
-  } else {
-    ComputeWeightHelper(p, sol, |sol[..|sol| - 1]| - 1);
-    assert computeWeight(p.weights, sol, |sol[..|sol| - 1]| - 1) == computeWeight(p.weights, sol[..|sol| - 1], |sol[..|sol| - 1]| - 1);
-  }
-}
-
-lemma emptySolutionIsOptimal(p: Problem, sol: seq<int>, i: int, j: int)
+lemma emptySolOptimal(p: Problem, solution: Solution, i: int, j: int)
  requires isValidProblem(p)
- requires 0 <= j <= p.knapsackCapacity
- requires |sol| == i == 0
- requires isPartialSolutionOfFirstIObjectsAndWeightJ(p, sol, i, j)
+ requires 0 <= j <= p.c
+ requires |solution| == i == 0
+ requires isPartialSolution(p, solution, i, j)
 
- ensures isOptimalPartialSolutionOfFirstIObjectsAndWeightJ(p, sol, i, j)
+ ensures isOptimalPartialSolution(p, solution, i, j)
 {
-  forall s: seq<int>  | isPartialSolutionOfFirstIObjectsAndWeightJ(p, s, i, j) && |sol| == |s|
-  ensures gain(p, sol) >= gain(p, s) 
+  forall s: Solution  | isPartialSolution(p, s, i, j) && |solution| == |s|
+  ensures gain(p, solution) >= gain(p, s) 
   { } 
-  assert forall s: seq<int> :: ((isPartialSolutionOfFirstIObjectsAndWeightJ(p, s, i, j) && |s| == |sol| ==> gain(p, sol) >= gain(p, s)));
+  assert forall s: Solution :: ((isPartialSolution(p, s, i, j) && |s| == |solution| ==> gain(p, solution) >= gain(p, s)));
 }
 
-lemma Weight0Lemma(p: Problem, sol: seq<int>, i: int)
+lemma ComputeWeightAllZeros(p: Problem, solution: Solution, i: int)
   requires isValidProblem(p)
-  requires 0 <= i < |sol|
+  requires 0 <= i < |solution|
   requires 0 <= i < |p.weights|
-  requires 0 <= |sol| <= p.numberOfObjects 
-  requires forall k :: 0 <= k < |sol| ==> sol[k] == 0
+  requires 0 <= |solution| <= p.n 
+  requires forall k :: 0 <= k < |solution| ==> solution[k] == 0
   
-  ensures computeWeight(p.weights, sol, i) == 0
+  ensures computeWeight(p.weights, solution, i) == 0
 {
   if i == 0 {
-    assert  computeWeight(p.weights, sol, i) == 0;
+    assert  computeWeight(p.weights, solution, i) == 0;
   } else {
-    Weight0Lemma(p, sol, i - 1);
-    assert computeWeight(p.weights, sol, i - 1) == 0;
-    assert computeWeight(p.weights, sol, i) == 0;
+    ComputeWeightAllZeros(p, solution, i - 1);
+    assert computeWeight(p.weights, solution, i - 1) == 0;
+    assert computeWeight(p.weights, solution, i) == 0;
   }
 }
 
-lemma Gain0Lemma(p: Problem, sol: seq<int>, i: int)
+lemma ComputeGainAllZeros(p: Problem, solution: Solution, i: int)
   requires isValidProblem(p)
-  requires 0 <= i < |sol|
+  requires 0 <= i < |solution|
   requires 0 <= i < |p.gains|
-  requires 0 <= |sol| <= p.numberOfObjects 
-  requires forall k :: 0 <= k < |sol| ==> sol[k] == 0
+  requires 0 <= |solution| <= p.n 
+  requires forall k :: 0 <= k < |solution| ==> solution[k] == 0
   
-  ensures computeGain(p.gains, sol, i) == 0
+  ensures computeGain(p.gains, solution, i) == 0
 {
   if i == 0 {
-    assert  computeGain(p.gains, sol, i) == 0;
+    assert  computeGain(p.gains, solution, i) == 0;
   } else {
-    Gain0Lemma(p, sol, i - 1);
-    assert computeGain(p.gains, sol, i - 1) == 0;
-    assert computeGain(p.gains, sol, i) == 0;
+    ComputeGainAllZeros(p, solution, i - 1);
+    assert computeGain(p.gains, solution, i - 1) == 0;
+    assert computeGain(p.gains, solution, i) == 0;
   }
 }
 
-lemma SubsolutionWeightIsZero(p: Problem, sol: seq<int>, i:int, j: int, idx: int, n : int)
+lemma {:induction false} ComputeWeightCapacity0(p: Problem, solution: Solution, i: int, idx: int, x: int)
  requires isValidProblem(p)
- requires 1 <= i <= p.numberOfObjects
- requires 0 <= |sol| <= p.numberOfObjects
- requires j == 0
- requires isPartialSolutionOfFirstIObjectsAndWeightJ(p, sol, i, j)
- requires 0 <= n <= |sol| - 1
- requires computeWeight(p.weights, sol, n) == 0
- requires 0 <= idx <= n
+ requires 1 <= i <= p.n
+ requires 0 <= |solution| <= p.n
+ requires isPartialSolution(p, solution, i, 0)
+ requires 0 <= x <= |solution| - 1
+ requires computeWeight(p.weights, solution, x) == 0
+ requires 0 <= idx <= x
  
- ensures computeWeight(p.weights, sol, idx) == 0
+ ensures computeWeight(p.weights, solution, idx) == 0
 {
-  if idx == n {
-    assert computeWeight(p.weights, sol, idx) == 0;
+  if idx == x {
+    assert computeWeight(p.weights, solution, idx) == 0;
   } else {
-    assert computeWeight(p.weights, sol, n - 1) == 0 by 
+    assert computeWeight(p.weights, solution, x - 1) == 0 by 
     {
-      assert n > 0;
-      assert 0 <= idx < n;
-      assert computeWeight(p.weights, sol, n) == 0;
-      assert p.weights[n] > 0;
-      assert 0 <= sol[n] <= 1;
-      assert sol[n] * p.weights[n] >= 0;
-      assert computeWeight(p.weights, sol, n) == sol[n] * p.weights[n] + computeWeight(p.weights, sol, n - 1);
+      assert x > 0;
+      assert 0 <= idx < x;
+      assert computeWeight(p.weights, solution, x) == 0;
+      assert p.weights[x] > 0;
+      assert 0 <= solution[x] <= 1;
+      assert solution[x] * p.weights[x] >= 0;
+      assert computeWeight(p.weights, solution, x) == solution[x] * p.weights[x] + computeWeight(p.weights, solution, x - 1);
     }
-    SubsolutionWeightIsZero(p, sol, i, j, idx, n - 1);
-    assert computeWeight(p.weights, sol, idx) == 0;
+    ComputeWeightCapacity0(p, solution, i, idx, x - 1);
+    assert computeWeight(p.weights, solution, idx) == 0;
   }
 }
 
-lemma Weight0ImpliesGain0(p: Problem, sol: seq<int>, i:int, j: int)
+lemma GainCapacity0(p: Problem, solution: Solution, i: int)
  requires isValidProblem(p)
- requires 1 <= i <= p.numberOfObjects
- requires |sol| == i
- requires j == 0
- requires isPartialSolutionOfFirstIObjectsAndWeightJ(p, sol, i, j)
- requires weight(p, sol) == 0
+ requires 1 <= i <= p.n
+ requires |solution| == i
+ requires isPartialSolution(p, solution, i, 0)
  
- ensures gain(p, sol) == 0
+ ensures gain(p, solution) == 0
 {
   var idx: int := 0;
-  while idx < |sol|
-    invariant 0 <= idx <= |sol|
-    invariant forall k :: 0 <= k < idx ==> sol[k] == 0
-    invariant idx > 0 ==> computeWeight(p.weights, sol, idx - 1) == 0
+  while idx < |solution|
+    invariant 0 <= idx <= |solution|
+    invariant forall k :: 0 <= k < idx ==> solution[k] == 0
+    invariant idx > 0 ==> computeWeight(p.weights, solution, idx - 1) == 0
   {
     assert p.weights[idx] > 0;
-    SubsolutionWeightIsZero(p, sol, i, j, idx, |sol| - 1);
-    assert p.weights[idx] > 0 && computeWeight(p.weights, sol, idx) == 0 ==> sol[idx] == 0;
+    ComputeWeightCapacity0(p, solution, i, idx, |solution| - 1);
+    assert p.weights[idx] > 0 && computeWeight(p.weights, solution, idx) == 0 ==> solution[idx] == 0;
     idx := idx + 1;
   }
-  assert forall k :: 0 <= k < |sol| ==> sol[k] == 0;
-  Gain0Lemma(p, sol, |sol| - 1);
-  assert gain(p, sol) == 0;
+  assert forall k :: 0 <= k < |solution| ==> solution[k] == 0;
+  ComputeGainAllZeros(p, solution, |solution| - 1);
+  assert gain(p, solution) == 0;
 }
 
-lemma MaximumWeightAllowedIs0(p: Problem, sol: seq<int>, i: int, j: int)
+lemma OptimalSolCapacity0(p: Problem, solution: Solution, i: int)
  requires isValidProblem(p)
- requires 1 <= i <= p.numberOfObjects
+ requires 1 <= i <= p.n
  requires 1 <= i <= |p.gains|
- requires j == 0
- requires isPartialSolutionOfFirstIObjectsAndWeightJ(p, sol, i, j)
- requires forall k :: 0 <= k < |sol| ==> sol[k] == 0
- requires weight(p, sol) == 0
+ requires isPartialSolution(p, solution, i, 0)
+ requires forall k :: 0 <= k < |solution| ==> solution[k] == 0
+ requires weight(p, solution) == 0
 
- ensures isOptimalPartialSolutionOfFirstIObjectsAndWeightJ(p, sol, i, j)
+ ensures isOptimalPartialSolution(p, solution, i, 0)
 {
-  assert isPartialSolutionOfFirstIObjectsAndWeightJ(p, sol, i, j);
-  forall s: seq<int> | isPartialSolutionOfFirstIObjectsAndWeightJ(p, s, i, j) && |sol| == |s|
-  ensures gain(p, sol) >= gain(p, s)
+  assert isPartialSolution(p, solution, i, 0);
+  forall s: Solution | isPartialSolution(p, s, i, 0) && |solution| == |s|
+  ensures gain(p, solution) >= gain(p, s)
   {
-    assert weight(p, sol) == 0 <= j;
-    assert forall k :: 0 <= k < |sol| ==> sol[k] == 0;
-    Gain0Lemma(p, sol, |sol| - 1);
-    Weight0ImpliesGain0(p, s, i, j);
-    assert gain(p, sol) == 0;
+    assert weight(p, solution) == 0;
+    assert forall k :: 0 <= k < |solution| ==> solution[k] == 0;
+    ComputeGainAllZeros(p, solution, |solution| - 1);
+    GainCapacity0(p, s, i);
+    assert gain(p, solution) == 0;
     assert gain(p, s) == 0;
   }
-  assert forall s: seq<int> :: (isPartialSolutionOfFirstIObjectsAndWeightJ(p, s, i, j) && |s| == |sol| ==> gain(p, sol) >= gain(p, s));
-  assert isOptimalPartialSolutionOfFirstIObjectsAndWeightJ(p, sol, i, j);
+  assert forall s: Solution :: (isPartialSolution(p, s, i, 0) && |s| == |solution| ==> gain(p, solution) >= gain(p, s));
+  assert isOptimalPartialSolution(p, solution, i, 0);
 }
 
-method KnapsackProblem(p: Problem) returns (profit: int, solution: seq<int>)
+lemma GainAdd0Optimal(p: Problem, profit1: int, profit2: int, solution1: Solution, solution2: Solution, x: Solution, i: int, j: int) //GainAdd0
+ requires isValidProblem(p)
+ requires 1 <= i <= p.n
+ requires 0 <= j <= p.c
+ requires p.weights[i - 1] <= j
+ requires isOptimalPartialSolution(p, solution1, i - 1, j - p.weights[i - 1])
+ requires isOptimalPartialSolution(p, solution2, i - 1, j)
+ requires computeWeight(p.weights, solution2 + [0], |solution2 + [0]| - 1) <= j
+ requires profit1 == gain(p, solution1)
+ requires profit2 == gain(p, solution2)
+ requires p.gains[i - 1] + profit1 <= profit2
+ requires isOptimalPartialSolution(p, x, i, j)
+ requires x[i - 1] == 0
+
+ ensures gain(p, x) == gain(p, solution2 + [0])
+{
+  var x' := x[..i - 1];
+  assert x' == x[..|x| - 1];
+  GainAdd0(p, x);
+  assert gain(p, x) == gain(p, x[..i - 1]) == gain(p, x');
+
+  OptimalSolRemove0(p, x, i, j);
+  assert isOptimalPartialSolution(p, x', i - 1, j);
+
+  assert gain(p, x') == gain(p, solution2);
+  
+  GainAdd0(p, solution2 + [0]);
+  assert gain(p, solution2) == gain(p, solution2 + [0]);
+
+  GainAdd0(p, x);
+  assert x == x' + [0];
+  assert gain(p, x' + [0]) == gain(p, x) == gain(p, solution2 + [0]);
+}
+
+lemma OptimalSolAdd0(p: Problem, profit1: int, profit2: int, solution1: Solution, solution2:Solution, i: int, j: int)
+                                    // profit1 = profits[i - 1][j - p.weights[i - 1]] 
+                                    // profit2 = profits[i - 1][j] 
+ requires isValidProblem(p)
+ requires 1 <= i <= p.n
+ requires 0 <= j <= p.c
+ requires p.weights[i - 1] <= j
+ requires isOptimalPartialSolution(p, solution1, i - 1, j - p.weights[i - 1])
+ requires isOptimalPartialSolution(p, solution2, i - 1, j)
+ requires computeWeight(p.weights, solution2 + [0], |solution2 + [0]| - 1) <= j
+ requires profit1 == gain(p, solution1)
+ requires profit2 == gain(p, solution2)
+ requires p.gains[i - 1] + profit1 <= profit2
+
+ ensures isOptimalPartialSolution(p, solution2 + [0], i, j)
+{
+  if !isOptimalPartialSolution(p, solution2 + [0], i, j) {
+    ExistsOptimalPartialSol(p, i, j);
+    var x : Solution :| isOptimalPartialSolution(p, x, i, j);
+
+    if x[i - 1] == 1 {
+      var x' := x[..i - 1];
+      assert gain(p, x') == profit1 by {
+        OptimalSolRemove1(p, x, i, j);
+        assert x' == x[..|x| - 1];
+        assert isOptimalPartialSolution(p, x', i - 1, j - p.weights[i - 1]);
+      }
+      GainAdd1(p, x);
+      GainAdd0(p, solution2 + [0]);
+      assert gain(p, x) == gain(p, x') + p.gains[i - 1] <= gain(p, solution2 + [0]);
+      assert false;
+    }
+    assert x[i - 1] == 0;
+    GainAdd0Optimal(p, profit1, profit2, solution1, solution2, x, i, j);
+    assert gain(p, x) == gain(p, solution2 + [0]);
+  }
+}
+
+lemma GainAddTooBig(p: Problem, solution: Solution, i: int, j: int)
+ requires isValidProblem(p)
+ requires 1 <= i <= p.n
+ requires 1 <= i <= |p.gains|
+ requires 1 <= j <= p.c
+ requires isPartialSolution(p, solution, i, j)
+ requires |solution| >= 2
+ requires p.weights[i - 1] > j
+
+ ensures solution[i - 1] == 0
+ ensures gain(p, solution[..i - 1]) == gain(p, solution)
+ {
+    if solution[i - 1] == 1 {
+      assert computeWeight(p.weights, solution, |solution| - 1) == computeWeight(p.weights, solution, |solution[..i]| - 1) + p.weights[i - 1];
+      assert weight(p, solution) >= p.weights[i - 1] > j;
+      assert !isPartialSolution(p, solution, i, j);
+      assert false;
+    }
+
+    assert solution[i - 1] == 0;
+    ComputeGainAdd0(p, solution, |solution| - 2);
+    assert gain(p, solution[..i - 1]) == gain(p, solution);
+}
+
+lemma GainUpperBound(p: Problem, solution: Solution, i: int) 
+ requires isValidProblem(p)
+ requires 1 <= i <= p.n
+ requires 0 <= |solution| <= |p.gains|
+ requires isValidPartialSolution(p, solution) && |solution| >= i 
+
+ ensures computeGainNew(p, solution, i - 1) <= SumAllGains(p, i)
+{
+  var completeSol := seq(i, y => 1);
+  assert forall q :: 0 <= q < i ==> completeSol[q] == 1;
+  var sumAllGains := computeGainNew(p, completeSol, |completeSol| - 1);
+  if i > 1 { 
+    GainUpperBound(p, solution, i - 1);
+    assert computeGainNew(p, solution, i - 2) <= SumAllGains(p, i - 1);
+  } else {
+  }
+}
+
+lemma ExistsOptimalPartialSol(p: Problem, i: int, j: int) 
+ requires isValidProblem(p)
+ requires 1 <= i <= p.n
+ requires 0 <= j <= p.c
+
+ ensures exists s :: isOptimalPartialSolution(p, s, i, j)
+{
+  var k : int := 0;
+  var completeSol := seq(i, y => 1);
+  assert forall q :: 0 <= q < i ==> completeSol[q] == 1;
+  var sumAllGains := SumAllGains(p, i);
+  assert forall k :: 0 <= k < i ==> p.gains[k] > 0;
+
+  if !exists s :: isOptimalPartialSolution(p, s, i, j) {
+    var q := 0; 
+    var currentSol := seq(i, y => 0);
+    ComputeWeightAllZeros(p, currentSol, |currentSol| - 1);
+    assert isPartialSolution(p, currentSol, i, j);
+    ComputeGainAllZeros(p, currentSol, |currentSol| - 1);
+    assert computeGain(p.gains, currentSol, |currentSol| - 1) == 0 >= q;
+    assert sumAllGains == SumAllGains(p, i);
+
+    while q < sumAllGains + 1
+      invariant 0 <= q <= sumAllGains + 1
+      invariant !exists s :: isOptimalPartialSolution(p, s, i, j)
+      invariant !isOptimalPartialSolution(p, currentSol, i, j)
+      invariant isPartialSolution(p, currentSol, i, j)
+      invariant computeGain(p.gains, currentSol, |currentSol| - 1) >= q
+    {
+      assert exists s_i :: isPartialSolution(p, s_i, i, j) && gain(p, s_i) > gain(p, currentSol);
+      var s_i :| isPartialSolution(p, s_i, i, j) && gain(p, s_i) > gain(p, currentSol);
+      
+      currentSol := s_i;
+      q := computeGain(p.gains, s_i, |s_i| - 1);
+      GainUpperBound(p, s_i, i);
+
+    }
+    
+    assert computeGainNew(p, currentSol, |currentSol| - 1) >= sumAllGains + 1;
+    GainUpperBound(p, currentSol, i);
+    assert false;
+  }
+}
+
+lemma OptimalSolAdd0TooBig(p: Problem, solution: Solution, i: int, j: int) //rename with j rel
+ requires isValidProblem(p)
+ requires 1 <= i <= p.n
+ requires 1 <= j <= p.c
+ requires isOptimalPartialSolution(p, solution, i - 1, j)
+ requires computeWeight(p.weights, solution + [0], |solution + [0]| - 1) <= j 
+ requires p.weights[i - 1] > j
+
+ ensures isOptimalPartialSolution(p, solution + [0], i, j)
+{
+  var s := solution + [0];
+  WeightAdd0(p, s);
+
+  if !isOptimalPartialSolution(p, s, i, j) {
+    assert isPartialSolution(p, s, i, j);
+    assert !isOptimalPartialSolution(p, s, i, j);
+    
+    ExistsOptimalPartialSol(p, i, j);
+    assert isValidProblem(p);
+    assert 1 <= i <= p.n;
+    assert 0 <= j <= p.c;
+    assert exists s :: isOptimalPartialSolution(p, s, i, j);
+
+    var x : Solution :| isOptimalPartialSolution(p, x, i, j);
+
+    GainAddTooBig(p, s, i, j);
+    assert gain(p, s[..i - 1]) == gain(p, s); 
+
+    GainAddTooBig(p, x, i, j);
+    var x1 := x[..i - 1];
+
+    assert gain(p, x1) == gain(p, x) > gain(p, s);  
+    assert gain(p, s) == gain(p, solution) < gain(p, x);
+    assert gain(p, x1) > gain(p, solution);
+    
+    assert isPartialSolution(p, x, i, j);
+    assert x[i - 1] == 0;
+    ComputeWeightAdd0(p, x, |x| - 2);
+    assert weight(p, x) == weight(p, x1);
+    assert isPartialSolution(p, x1, i - 1, j);
+    assert !isOptimalPartialSolution(p, solution, i - 1, j);
+    assert false;
+  }
+}
+
+lemma OptimalSolRemove1(p: Problem, solution: Solution, i: int, j: int)
+ requires isValidProblem(p)
+ requires 1 <= i <= p.n
+ requires 0 <= j <= p.c
+ requires isOptimalPartialSolution(p, solution, i, j)
+ requires solution[i - 1] == 1
+
+ ensures isOptimalPartialSolution(p, solution[..i - 1], i - 1, j - p.weights[i - 1])
+{
+  var s' := solution[..i - 1];
+  WeightAdd1(p, solution);
+  assert isPartialSolution(p, solution[..i - 1], i - 1, j - p.weights[i - 1]);
+
+  if !isOptimalPartialSolution(p, solution[..i - 1], i - 1, j - p.weights[i - 1]) {
+    GainAdd1(p, solution);
+    ExistsOptimalPartialSol(p, i - 1, j - p.weights[i - 1]);
+    var x : Solution :| isOptimalPartialSolution(p, x, i - 1, j - p.weights[i - 1]);
+    assert |x| == |solution[..i - 1]|;
+    assert gain(p, x) > gain(p, solution[..i - 1]);
+
+    var x1 := x + [1];
+    GainAdd1(p, x1);
+    WeightAdd1(p, x1);
+    assert isOptimalPartialSolution(p, x1, i, j);
+    assert s' == solution[..|solution| - 1];
+    assert x == x1[..|x1| - 1];
+    assert gain(p, x1) == gain(p, x) + p.gains[i - 1] > gain(p, s') + p.gains[i- 1] == gain(p, solution);
+    assert gain(p, x1) > gain(p, solution);
+    assert false;
+  }
+}
+
+lemma OptimalSolRemove0(p: Problem, solution: Solution, i: int, j: int)
+ requires isValidProblem(p)
+ requires 1 <= i <= p.n
+ requires 0 <= j <= p.c
+ requires isOptimalPartialSolution(p, solution, i, j)
+ requires solution[i - 1] == 0
+
+ ensures isOptimalPartialSolution(p, solution[..i - 1], i - 1, j)
+{
+  var s' := solution[..i - 1];
+  WeightAdd0(p, solution);
+  assert isPartialSolution(p, solution[..i - 1], i - 1, j);
+
+  if !isOptimalPartialSolution(p, solution[..i - 1], i - 1, j) {
+    GainAdd0(p, solution);
+    ExistsOptimalPartialSol(p, i - 1, j);
+    var x : Solution :| isOptimalPartialSolution(p, x, i - 1, j);
+    assert |x| == |solution[..i - 1]|;
+
+    var x1 := x + [0];
+    GainAdd0(p, x1);
+    WeightAdd0(p, x1);
+    assert isOptimalPartialSolution(p, x1, i, j);
+    assert s' == solution[..|solution| - 1];
+    assert x == x1[..|x1| - 1];
+    assert gain(p, x1) == gain(p, x) >= gain(p, s') == gain(p, solution);
+    assert gain(p, x1) == gain(p, solution);
+    assert false;
+  }
+}
+
+lemma GainAdd1Optimal(p: Problem, profit1: int, profit2: int, solution1: Solution, solution2: Solution, x: Solution, i: int, j: int)
+ requires isValidProblem(p)
+ requires 1 <= i <= p.n
+ requires 0 <= j <= p.c
+ requires p.weights[i - 1] <= j
+ requires isOptimalPartialSolution(p, solution1, i - 1, j - p.weights[i - 1])
+ requires isOptimalPartialSolution(p, solution2, i - 1, j)
+ requires computeWeight(p.weights, solution1 + [1], |solution1 + [1]| - 1) <= j
+ requires p.gains[i - 1] + profit1 > profit2
+ requires isOptimalPartialSolution(p, x, i, j)
+ requires x[i - 1] == 1
+
+ ensures gain(p, x) == gain(p, solution1 + [1])
+{
+   assert gain(p, x) == gain(p, solution1 + [1]) by { 
+      GainAdd1(p, solution1 + [1]);
+      GainAdd1(p, x);
+      assert x == x[..i - 1] + [1];
+      assert gain(p, x[..i - 1]) == gain(p, solution1) by
+      {
+        OptimalSolRemove1(p, x, i, j);
+        assert isOptimalPartialSolution(p, x[..i - 1], i - 1, j - p.weights[i - 1]);
+      } 
+  }
+}
+
+lemma OptimalSolAdd1(p: Problem, profit1: int, profit2: int, solution1: Solution, solution2: Solution, i: int, j: int)
+                                    // profit1 = profits[i - 1][j - p.weights[i - 1]] 
+                                    // profit2 = profits[i - 1][j] 
+ requires isValidProblem(p)
+ requires 1 <= i <= p.n
+ requires 0 <= j <= p.c
+ requires p.weights[i - 1] <= j
+ requires isOptimalPartialSolution(p, solution1, i - 1, j - p.weights[i - 1])
+ requires isOptimalPartialSolution(p, solution2, i - 1, j)
+ requires computeWeight(p.weights, solution1 + [1], |solution1 + [1]| - 1) <= j
+ requires profit1 == gain(p, solution1)
+ requires profit2 == gain(p, solution2)
+ requires p.gains[i - 1] + profit1 > profit2
+
+ ensures isOptimalPartialSolution(p, solution1 + [1], i, j)
+{
+  var s := solution1 + [1];
+
+  if !isOptimalPartialSolution(p, s, i, j){
+    ExistsOptimalPartialSol(p, i, j);
+
+    var x : seq<int> :| isOptimalPartialSolution(p, x, i, j);
+    assert gain(p, x) > gain(p, solution1 + [1]);
+    if x[i - 1] == 0 {
+      assert gain(p, x) <= profit2 by 
+      {
+        GainAdd0(p, x);
+        assert gain(p, x[..i - 1]) == gain(p, x);
+        WeightAdd0(p, x);
+        assert weight(p, x) <= j;
+        assert weight(p, x[..i - 1]) <= j;
+      }
+      assert gain(p, solution1 + [1]) > profit2 by 
+      {
+        GainAdd1(p, solution1 + [1]);
+        assert gain(p, solution1 + [1]) == gain(p, solution1) + p.gains[i - 1];
+      }
+      assert false; 
+    } else {
+      GainAdd1Optimal(p, profit1, profit2, solution1, solution2, x, i, j);
+      assert gain(p, x) == gain(p, solution1 + [1]);
+    }
+  }
+}
+
+method Solve(p: Problem) returns (profit: int, solution: Solution)
   requires isValidProblem(p)
   
   ensures isSolution(p, solution)
@@ -415,34 +743,34 @@ method KnapsackProblem(p: Problem) returns (profit: int, solution: seq<int>)
     var solutions := [];
     var i := 0;
 
-    var partialProfits, partialSolutions := FillMatrixForObject0(p, profits, solutions, i);
+    var partialProfits, partialSolutions := Solves0Objects(p, profits, solutions, i);
     profits := profits + [partialProfits];
     solutions := solutions + [partialSolutions];
-    assert forall k :: 0 <= k < |solutions| ==> forall q :: 0 <= q < |solutions[k]| ==> weight(p, solutions[k][q]) <= q;
+    assert forall k :: 0 <= k < |solutions| ==> forall q :: 0 <= q < |solutions[k]| ==> weight(p, solutions[k][q]) <= q; // de vazut care trebuie sa ramana
     assert forall k :: 0 <= k < |solutions| ==> forall q :: 0 <= q < |solutions[k]| ==> |solutions[k][q]| == i;
-    assert forall k :: 0 <= k < |partialSolutions| ==> isPartialSolutionOfFirstIObjectsAndWeightJ(p, partialSolutions[k], i, k);
+    assert forall k :: 0 <= k < |partialSolutions| ==> isPartialSolution(p, partialSolutions[k], i, k);
 
-    assert forall k :: 0 <= k < |partialSolutions| ==> isOptimalPartialSolutionOfFirstIObjectsAndWeightJ(p, partialSolutions[k], i ,k);
+    assert forall k :: 0 <= k < |partialSolutions| ==> isOptimalPartialSolution(p, partialSolutions[k], i ,k);
     assert forall k :: 0 <= k < |solutions| ==> forall q :: 0 <= q < |solutions[k]| ==> gain(p, solutions[k][q]) == profits[k][q];
 
     i := i + 1;
 
-    while i <= p.numberOfObjects 
-      invariant |profits| == |solutions| == i
-      invariant 0 <= i <= p.numberOfObjects + 1
-      invariant forall k :: 0 <= k < i ==> |profits[k]| == p.knapsackCapacity + 1
-      invariant 0 <= |profits| <= p.numberOfObjects + 1
+    while i <= p.n 
+      invariant |profits| == |solutions| == i // de vazut care trebuie sa ramana
+      invariant 0 <= i <= p.n + 1
+      invariant forall k :: 0 <= k < i ==> |profits[k]| == p.c + 1
+      invariant 0 <= |profits| <= p.n + 1
 
-      invariant forall k :: 0 <= k < |solutions| ==> |solutions[k]| == p.knapsackCapacity + 1
+      invariant forall k :: 0 <= k < |solutions| ==> |solutions[k]| == p.c + 1
       invariant forall k :: 0 <= k < |solutions| ==> forall q :: 0 <= q < |solutions[k]| ==> |solutions[k][q]| == k
-      invariant forall k :: 0 <= k < |solutions| ==> forall q :: 0 <= q < |solutions[k]| ==> hasOnlyPermittedValues(solutions[k][q])
-      invariant forall k :: 0 <= k < i ==> forall q :: 0 <= q < |solutions[k]| ==> 0 <= |solutions[k][q]| <= p.numberOfObjects
+      invariant forall k :: 0 <= k < |solutions| ==> forall q :: 0 <= q < |solutions[k]| ==> hasAllowedValues(solutions[k][q])
+      invariant forall k :: 0 <= k < i ==> forall q :: 0 <= q < |solutions[k]| ==> 0 <= |solutions[k][q]| <= p.n
 
       invariant forall k :: 0 <= k < |solutions| ==> forall q :: 0 <= q < |solutions[k]| ==> 
-                        isPartialSolutionOfFirstIObjectsAndWeightJ(p, solutions[k][q], k, q)
+                        isPartialSolution(p, solutions[k][q], k, q)
 
       invariant forall k :: 0 <= k < |solutions| ==> forall q :: 0 <= q < |solutions[k]| ==> 
-                isOptimalPartialSolutionOfFirstIObjectsAndWeightJ(p, solutions[k][q], k, q)
+                isOptimalPartialSolution(p, solutions[k][q], k, q)
       invariant forall k :: 0 <= k < |solutions| ==> forall q :: 0 <= q < |solutions[k]| ==> 
                 gain(p, solutions[k][q]) == profits[k][q]
     {
@@ -458,30 +786,27 @@ method KnapsackProblem(p: Problem) returns (profit: int, solution: seq<int>)
       print "\n";
     }
     
-    solution := solutions[p.numberOfObjects][p.knapsackCapacity];
-    assert weight(p, solution) <= p.knapsackCapacity;
-    assert isPartialSolution(p, solution);
+    solution := solutions[p.n][p.c];
+    assert weight(p, solution) <= p.c; // de vazut care trebuie sa ramana
     assert isSolution(p, solution);
-
-    assert isOptimalPartialSolution(p, solution);
     assert isOptimalSolution(p, solution);
 
-    profit := profits[p.numberOfObjects][p.knapsackCapacity];
+    profit := profits[p.n][p.c];
 }
 
-method FillMatrixForObject0(p: Problem, profits: seq<seq<int>>, solutions : seq<seq<seq<int>>>, i: int) returns (partialProfits: seq<int>, partialSolutions: seq<seq<int>>)
+method Solves0Objects(p: Problem, profits: seq<seq<int>>, solutions : seq<seq<seq<int>>>, i: int) returns (partialProfits: seq<int>, partialSolutions: seq<seq<int>>)
   requires isValidProblem(p)
   requires |profits| == |solutions| == i == 0
 
-  ensures |partialProfits| == p.knapsackCapacity + 1
-  ensures |partialSolutions| == p.knapsackCapacity + 1
+  ensures |partialProfits| == p.c + 1 // de vazut care trebuie sa ramana
+  ensures |partialSolutions| == p.c + 1
   ensures forall k :: 0 <= k < |partialSolutions| ==> |partialSolutions[k]| == i
-  ensures forall k :: 0 <= k < |partialSolutions| ==> hasOnlyPermittedValues(partialSolutions[k])
+  ensures forall k :: 0 <= k < |partialSolutions| ==> hasAllowedValues(partialSolutions[k])
   ensures forall k :: 0 <= k < |partialSolutions| ==> weight(p, partialSolutions[k]) <= k
   ensures forall k :: 0 <= k < |partialSolutions| ==> forall q :: 0 <= q < |partialSolutions[k]| ==> partialSolutions[k][q] == 0
-  ensures forall k :: 0 <= k < |partialSolutions| ==> isPartialSolutionOfFirstIObjectsAndWeightJ(p, partialSolutions[k], i, k)
+  ensures forall k :: 0 <= k < |partialSolutions| ==> isPartialSolution(p, partialSolutions[k], i, k)
 
-  ensures forall k :: 0 <= k < |partialSolutions| ==> isOptimalPartialSolutionOfFirstIObjectsAndWeightJ(p, partialSolutions[k], i, k)
+  ensures forall k :: 0 <= k < |partialSolutions| ==> isOptimalPartialSolution(p, partialSolutions[k], i, k)
   ensures forall k :: 0 <= k < |partialSolutions| ==> gain(p, partialSolutions[k]) == partialProfits[k]
 {
         partialProfits := [];
@@ -491,24 +816,24 @@ method FillMatrixForObject0(p: Problem, profits: seq<seq<int>>, solutions : seq<
 
         assert weight(p, currentSolution) == 0;
 
-         while j <= p.knapsackCapacity
-          invariant 0 <= j <= p.knapsackCapacity + 1
+         while j <= p.c
+          invariant 0 <= j <= p.c + 1 // de vazut care trebuie sa ramana
           invariant |partialProfits| == j
           invariant |partialSolutions| == j
 
           invariant |partialSolutions| > 0 ==> forall k :: 0 <= k < |partialSolutions| ==> |partialSolutions[k]| == i 
-          invariant forall k :: 0 <= k < |partialSolutions| ==> hasOnlyPermittedValues(partialSolutions[k])
+          invariant forall k :: 0 <= k < |partialSolutions| ==> hasAllowedValues(partialSolutions[k])
           invariant forall k :: 0 <= k < |partialSolutions| ==> weight(p, partialSolutions[k]) <= k
           invariant forall k :: 0 <= k < |partialSolutions| ==> forall q :: 0 <= q < |partialSolutions[k]| ==> partialSolutions[k][q] == 0
-          invariant forall k :: 0 <= k < |partialSolutions| ==> isPartialSolutionOfFirstIObjectsAndWeightJ(p, partialSolutions[k], i, k)
+          invariant forall k :: 0 <= k < |partialSolutions| ==> isPartialSolution(p, partialSolutions[k], i, k)
 
-          invariant forall k :: 0 <= k < |partialSolutions| ==> isOptimalPartialSolutionOfFirstIObjectsAndWeightJ(p, partialSolutions[k], i, k)
+          invariant forall k :: 0 <= k < |partialSolutions| ==> isOptimalPartialSolution(p, partialSolutions[k], i, k)
           invariant forall k :: 0 <= k < |partialSolutions| ==> gain(p, partialSolutions[k]) == partialProfits[k]
         {
               partialProfits := partialProfits + [0];
               currentSolution := [];
-              emptySolutionIsOptimal(p, currentSolution, i, j);
-              assert isOptimalPartialSolutionOfFirstIObjectsAndWeightJ(p, currentSolution, i, j);
+              emptySolOptimal(p, currentSolution, i, j);
+              assert isOptimalPartialSolution(p, currentSolution, i, j);
               partialSolutions := partialSolutions + [currentSolution];
 
               assert |currentSolution| == i;
@@ -518,429 +843,83 @@ method FillMatrixForObject0(p: Problem, profits: seq<seq<int>>, solutions : seq<
         }
 }
 
-lemma NotAddingObjectHasSameGainAsOptimalSol(p: Problem, profit1: int, profit2: int, sol1: seq<int>, sol2:seq<int>, x: seq<int>, i: int, j: int)
- requires isValidProblem(p)
- requires 1 <= i <= p.numberOfObjects
- requires 0 <= j <= p.knapsackCapacity
- requires p.weights[i - 1] <= j
- requires isOptimalPartialSolutionOfFirstIObjectsAndWeightJ(p, sol1, i - 1, j - p.weights[i - 1])
- requires isOptimalPartialSolutionOfFirstIObjectsAndWeightJ(p, sol2, i - 1, j)
- requires computeWeight(p.weights, sol2 + [0], |sol2 + [0]| - 1) <= j
- requires profit1 == gain(p, sol1)
- requires profit2 == gain(p, sol2)
- requires p.gains[i - 1] + profit1 <= profit2
- requires isOptimalPartialSolutionOfFirstIObjectsAndWeightJ(p, x, i, j)
- requires x[i - 1] == 0
-
- ensures gain(p, x) == gain(p, sol2 + [0])
-{
-  var x' := x[..i - 1];
-  assert x' == x[..|x| - 1];
-  LastElementIs0ForGainHelper(p, x);
-  assert gain(p, x) == gain(p, x[..i - 1]) == gain(p, x');
-
-  OptimalSubsolutionForLastElement0(p, x, i, j);
-  assert isOptimalPartialSolutionOfFirstIObjectsAndWeightJ(p, x', i - 1, j);
-
-  assert gain(p, x') == gain(p, sol2);
-  
-  LastElementIs0ForGainHelper(p, sol2 + [0]);
-  assert gain(p, sol2) == gain(p, sol2 + [0]);
-
-  LastElementIs0ForGainHelper(p, x);
-  assert x == x' + [0];
-  assert gain(p, x' + [0]) == gain(p, x) == gain(p, sol2 + [0]);
-}
-
-lemma NotTakingObjectLeadsToOptimalCase1(p: Problem, profit1: int, profit2: int, sol1: seq<int>, sol2:seq<int>, i: int, j: int) 
-                                    // profit1 = profits[i - 1][j - p.weights[i - 1]] 
-                                    // profit2 = profits[i - 1][j] 
- requires isValidProblem(p)
- requires 1 <= i <= p.numberOfObjects
- requires 0 <= j <= p.knapsackCapacity
- requires p.weights[i - 1] <= j
- requires isOptimalPartialSolutionOfFirstIObjectsAndWeightJ(p, sol1, i - 1, j - p.weights[i - 1])
- requires isOptimalPartialSolutionOfFirstIObjectsAndWeightJ(p, sol2, i - 1, j)
- requires computeWeight(p.weights, sol2 + [0], |sol2 + [0]| - 1) <= j
- requires profit1 == gain(p, sol1)
- requires profit2 == gain(p, sol2)
- requires p.gains[i - 1] + profit1 <= profit2
-
- ensures isOptimalPartialSolutionOfFirstIObjectsAndWeightJ(p, sol2 + [0], i, j)
-{
-  if !isOptimalPartialSolutionOfFirstIObjectsAndWeightJ(p, sol2 + [0], i, j) {
-    ExistsOptimalPartialSolution(p, i, j);
-    var x : seq<int> :| isOptimalPartialSolutionOfFirstIObjectsAndWeightJ(p, x, i, j);
-
-    if x[i - 1] == 1 {
-      var x' := x[..i - 1];
-      assert gain(p, x') == profit1 by {
-        OptimalSubsolutionForLastElement1(p, x, i, j);
-        assert x' == x[..|x| - 1];
-        assert isOptimalPartialSolutionOfFirstIObjectsAndWeightJ(p, x', i - 1, j - p.weights[i - 1]);
-      }
-      LastElementIs1ForGainHelper(p, x);
-      LastElementIs0ForGainHelper(p, sol2 + [0]);
-      assert gain(p, x) == gain(p, x') + p.gains[i - 1] <= gain(p, sol2 + [0]);
-      assert false;
-    }
-    assert x[i - 1] == 0;
-    NotAddingObjectHasSameGainAsOptimalSol(p, profit1, profit2, sol1, sol2, x, i, j);
-    assert gain(p, x) == gain(p, sol2 + [0]);
-  }
-}
-
-lemma LastElemIs0AndGainIsUnchanged(p: Problem, sol: seq<int>, i: int, j: int)
- requires isValidProblem(p)
- requires 1 <= i <= p.numberOfObjects
- requires 1 <= i <= |p.gains|
- requires 1 <= j <= p.knapsackCapacity
- requires isPartialSolutionOfFirstIObjectsAndWeightJ(p, sol, i, j)
- requires |sol| >= 2
- requires p.weights[i - 1] > j
-
- ensures sol[i - 1] == 0
- ensures gain(p, sol[..i - 1]) == gain(p, sol)
- {
-    if sol[i - 1] == 1 {
-      assert computeWeight(p.weights, sol, |sol| - 1) == computeWeight(p.weights, sol, |sol[..i]| - 1) + p.weights[i - 1];
-      assert weight(p, sol) >= p.weights[i - 1] > j;
-      assert !isPartialSolutionOfFirstIObjectsAndWeightJ(p, sol, i, j);
-      assert false;
-    }
-
-    assert sol[i - 1] == 0;
-    LastElementIs0ForComputeGainHelper(p, sol, |sol| - 2);
-    assert gain(p, sol[..i - 1]) == gain(p, sol);
-}
-
-function MaximumGain(p: Problem, i: int) : int
- requires isValidProblem(p)
- requires 1 <= i <= p.numberOfObjects
-
- ensures MaximumGain(p, i) >= 0
-{
-  if (i == 1) then p.gains[0] else p.gains[i - 1] + MaximumGain(p, i -1)
-}
-
-lemma GainUpperBound(p: Problem, i: int, s: seq<int>) 
- requires isValidProblem(p)
- requires 1 <= i <= p.numberOfObjects
- requires 0 <= |s| <= |p.gains|
- requires isValidPartialSolution(p, s) && |s| >= i 
-
- ensures computeGainNew(p, s, i - 1) <= MaximumGain(p, i)
-{
-  var completeSol := seq(i, w => 1);
-  assert forall q :: 0 <= q < i ==> completeSol[q] == 1;
-  var sumAllGains := computeGainNew(p, completeSol, |completeSol| - 1);
-  if i > 1 { 
-    GainUpperBound(p, i - 1, s);
-    assert computeGainNew(p, s, i - 2) <= MaximumGain(p, i - 1);
-  } else {
-  }
-}
-
-lemma ExistsOptimalPartialSolution(p: Problem, i: int, j: int) 
- requires isValidProblem(p)
- requires 1 <= i <= p.numberOfObjects
- requires 0 <= j <= p.knapsackCapacity
-
- ensures exists s :: isOptimalPartialSolutionOfFirstIObjectsAndWeightJ(p, s, i, j)
-{
-  var k : int := 0;
-  var completeSol := seq(i, w => 1);
-  assert forall q :: 0 <= q < i ==> completeSol[q] == 1;
-  var sumAllGains := MaximumGain(p, i);
-  assert forall k :: 0 <= k < i ==> p.gains[k] > 0;
-
-  if !exists s :: isOptimalPartialSolutionOfFirstIObjectsAndWeightJ(p, s, i, j) {
-    var q := 0; 
-    var currentSol := seq(i, w => 0);
-    Weight0Lemma(p, currentSol, |currentSol| - 1);
-    assert isPartialSolutionOfFirstIObjectsAndWeightJ(p, currentSol, i, j);
-    Gain0Lemma(p, currentSol, |currentSol| - 1);
-    assert computeGain(p.gains, currentSol, |currentSol| - 1) == 0 >= q;
-    assert sumAllGains == MaximumGain(p, i);
-
-    while q < sumAllGains + 1
-      invariant 0 <= q <= sumAllGains + 1
-      invariant !exists s :: isOptimalPartialSolutionOfFirstIObjectsAndWeightJ(p, s, i, j)
-      invariant !isOptimalPartialSolutionOfFirstIObjectsAndWeightJ(p, currentSol, i, j)
-      invariant isPartialSolutionOfFirstIObjectsAndWeightJ(p, currentSol, i, j)
-      invariant computeGain(p.gains, currentSol, |currentSol| - 1) >= q
-    {
-      assert exists s_i :: isPartialSolutionOfFirstIObjectsAndWeightJ(p, s_i, i, j) && gain(p, s_i) > gain(p, currentSol);
-      var s_i :| isPartialSolutionOfFirstIObjectsAndWeightJ(p, s_i, i, j) && gain(p, s_i) > gain(p, currentSol);
-      
-      currentSol := s_i;
-      q := computeGain(p.gains, s_i, |s_i| - 1);
-      GainUpperBound(p, i,  s_i);
-
-    }
-    
-    assert computeGainNew(p, currentSol, |currentSol| - 1) >= sumAllGains + 1;
-    GainUpperBound(p, i,  currentSol);
-    assert false;
-  }
-}
-
-lemma NotTakingObjectLeadsToOptimalCase2(p: Problem, sol: seq<int>, i: int, j: int) // sol is solutions[i - 1][j]
- requires isValidProblem(p)
- requires 1 <= i <= p.numberOfObjects
- requires 1 <= j <= p.knapsackCapacity
- requires isOptimalPartialSolutionOfFirstIObjectsAndWeightJ(p, sol, i - 1, j)
- requires computeWeight(p.weights, sol + [0], |sol + [0]| - 1) <= j 
- requires p.weights[i - 1] > j
-
- ensures isOptimalPartialSolutionOfFirstIObjectsAndWeightJ(p, sol + [0], i, j)
-{
-  var s := sol + [0];
-  LastElementIs0ForWeightHelper(p, s);
-
-  if !isOptimalPartialSolutionOfFirstIObjectsAndWeightJ(p, s, i, j) {
-    assert isPartialSolutionOfFirstIObjectsAndWeightJ(p, s, i, j);
-    assert !isOptimalPartialSolutionOfFirstIObjectsAndWeightJ(p, s, i, j);
-    
-    ExistsOptimalPartialSolution(p, i, j);
-    assert isValidProblem(p);
-    assert 1 <= i <= p.numberOfObjects;
-    assert 0 <= j <= p.knapsackCapacity;
-    assert exists s :: isOptimalPartialSolutionOfFirstIObjectsAndWeightJ(p, s, i, j);
-
-    var x : seq<int> :| isOptimalPartialSolutionOfFirstIObjectsAndWeightJ(p, x, i, j);
-
-    LastElemIs0AndGainIsUnchanged(p, s, i, j);
-    assert gain(p, s[..i - 1]) == gain(p, s); 
-
-    LastElemIs0AndGainIsUnchanged(p, x, i, j);
-    var x1 := x[..i - 1];
-
-    assert gain(p, x1) == gain(p, x) > gain(p, s);  
-    assert gain(p, s) == gain(p, sol) < gain(p, x);
-    assert gain(p, x1) > gain(p, sol);
-    
-    assert isPartialSolutionOfFirstIObjectsAndWeightJ(p, x, i, j);
-    assert x[i - 1] == 0;
-    LastElementIs0ForComputeWeightHelper(p, x, |x| - 2);
-    assert weight(p, x) == weight(p, x1);
-    assert isPartialSolutionOfFirstIObjectsAndWeightJ(p, x1, i - 1, j);
-    assert !isOptimalPartialSolutionOfFirstIObjectsAndWeightJ(p, sol, i - 1, j);
-    assert false;
-  }
-}
-
-lemma OptimalSubsolutionForLastElement1(p: Problem, s: seq<int>, i: int, j: int)
- requires isValidProblem(p)
- requires 1 <= i <= p.numberOfObjects
- requires 0 <= j <= p.knapsackCapacity
- requires isOptimalPartialSolutionOfFirstIObjectsAndWeightJ(p, s, i, j)
- requires s[i - 1] == 1
-
- ensures isOptimalPartialSolutionOfFirstIObjectsAndWeightJ(p, s[..i - 1], i - 1, j - p.weights[i - 1])
-{
-   var s' := s[..i - 1];
-  LastElementIs1ForWeightHelper(p, s);
-  assert isPartialSolutionOfFirstIObjectsAndWeightJ(p, s[..i - 1], i - 1, j - p.weights[i - 1]);
-
-  if !isOptimalPartialSolutionOfFirstIObjectsAndWeightJ(p, s[..i - 1], i - 1, j - p.weights[i - 1]) {
-    LastElementIs1ForGainHelper(p, s);
-    ExistsOptimalPartialSolution(p, i - 1, j - p.weights[i - 1]);
-    var x : seq<int> :| isOptimalPartialSolutionOfFirstIObjectsAndWeightJ(p, x, i - 1, j - p.weights[i - 1]);
-    assert |x| == |s[..i - 1]|;
-    assert gain(p, x) > gain(p, s[..i - 1]);
-
-    var x1 := x + [1];
-    LastElementIs1ForGainHelper(p, x1);
-    LastElementIs1ForWeightHelper(p, x1);
-    assert isOptimalPartialSolutionOfFirstIObjectsAndWeightJ(p, x1, i, j);
-    assert s' == s[..|s| - 1];
-    assert x == x1[..|x1| - 1];
-    assert gain(p, x1) == gain(p, x) + p.gains[i - 1] > gain(p, s') + p.gains[i- 1] == gain(p, s);
-    assert gain(p, x1) > gain(p, s);
-    assert false;
-  }
-}
-
-lemma OptimalSubsolutionForLastElement0(p: Problem, s: seq<int>, i: int, j: int)
- requires isValidProblem(p)
- requires 1 <= i <= p.numberOfObjects
- requires 0 <= j <= p.knapsackCapacity
- requires isOptimalPartialSolutionOfFirstIObjectsAndWeightJ(p, s, i, j)
- requires s[i - 1] == 0
-
- ensures isOptimalPartialSolutionOfFirstIObjectsAndWeightJ(p, s[..i - 1], i - 1, j)
-{
-   var s' := s[..i - 1];
-  LastElementIs0ForWeightHelper(p, s);
-  assert isPartialSolutionOfFirstIObjectsAndWeightJ(p, s[..i - 1], i - 1, j);
-
-  if !isOptimalPartialSolutionOfFirstIObjectsAndWeightJ(p, s[..i - 1], i - 1, j) {
-    LastElementIs0ForGainHelper(p, s);
-    ExistsOptimalPartialSolution(p, i - 1, j);
-    var x : seq<int> :| isOptimalPartialSolutionOfFirstIObjectsAndWeightJ(p, x, i - 1, j);
-    assert |x| == |s[..i - 1]|;
-
-    var x1 := x + [0];
-    LastElementIs0ForGainHelper(p, x1);
-    LastElementIs0ForWeightHelper(p, x1);
-    assert isOptimalPartialSolutionOfFirstIObjectsAndWeightJ(p, x1, i, j);
-    assert s' == s[..|s| - 1];
-    assert x == x1[..|x1| - 1];
-    assert gain(p, x1) == gain(p, x) >= gain(p, s') == gain(p, s);
-    assert gain(p, x1) == gain(p, s);
-    assert false;
-  }
-}
-
-lemma AddingObjHasEqualGainAsOptimalSol(p: Problem, profit1: int, profit2: int, sol1: seq<int>, sol2:seq<int>, x: seq<int>, i: int, j: int)
- requires isValidProblem(p)
- requires 1 <= i <= p.numberOfObjects
- requires 0 <= j <= p.knapsackCapacity
- requires p.weights[i - 1] <= j
- requires isOptimalPartialSolutionOfFirstIObjectsAndWeightJ(p, sol1, i - 1, j - p.weights[i - 1])
- requires isOptimalPartialSolutionOfFirstIObjectsAndWeightJ(p, sol2, i - 1, j)
- requires computeWeight(p.weights, sol1 + [1], |sol1 + [1]| - 1) <= j
- requires p.gains[i - 1] + profit1 > profit2
- requires isOptimalPartialSolutionOfFirstIObjectsAndWeightJ(p, x, i, j)
- requires x[i - 1] == 1
-
- ensures gain(p, x) == gain(p, sol1 + [1])
-{
-   assert gain(p, x) == gain(p, sol1 + [1]) by { 
-      LastElementIs1ForGainHelper(p, sol1 + [1]);
-      LastElementIs1ForGainHelper(p, x);
-      assert x == x[..i - 1] + [1];
-      assert gain(p, x[..i - 1]) == gain(p, sol1) by
-      {
-        OptimalSubsolutionForLastElement1(p, x, i, j);
-        assert isOptimalPartialSolutionOfFirstIObjectsAndWeightJ(p, x[..i - 1], i - 1, j - p.weights[i - 1]);
-      } 
-  }
-}
-
-lemma CaseTakingObjectLeadsToOptimal(p: Problem, profit1: int, profit2: int, sol1: seq<int>, sol2:seq<int>, i: int, j: int) 
-                                    // profit1 = profits[i - 1][j - p.weights[i - 1]] 
-                                    // profit2 = profits[i - 1][j] 
- requires isValidProblem(p)
- requires 1 <= i <= p.numberOfObjects
- requires 0 <= j <= p.knapsackCapacity
- requires p.weights[i - 1] <= j
- requires isOptimalPartialSolutionOfFirstIObjectsAndWeightJ(p, sol1, i - 1, j - p.weights[i - 1])
- requires isOptimalPartialSolutionOfFirstIObjectsAndWeightJ(p, sol2, i - 1, j)
- requires computeWeight(p.weights, sol1 + [1], |sol1 + [1]| - 1) <= j
- requires profit1 == gain(p, sol1)
- requires profit2 == gain(p, sol2)
- requires p.gains[i - 1] + profit1 > profit2
-
- ensures isOptimalPartialSolutionOfFirstIObjectsAndWeightJ(p, sol1 + [1], i, j)
-{
-  var s := sol1 + [1];
-
-  if !isOptimalPartialSolutionOfFirstIObjectsAndWeightJ(p, s, i, j){
-    ExistsOptimalPartialSolution(p, i, j);
-
-    var x : seq<int> :| isOptimalPartialSolutionOfFirstIObjectsAndWeightJ(p, x, i, j);
-    assert gain(p, x) > gain(p, sol1 + [1]);
-    if x[i - 1] == 0 {
-      assert gain(p, x) <= profit2 by // <= profits[i - 1][j]
-      {
-        LastElementIs0ForGainHelper(p, x);
-        assert gain(p, x[..i - 1]) == gain(p, x);
-        LastElementIs0ForWeightHelper(p, x);
-        assert weight(p, x) <= j;
-        assert weight(p, x[..i - 1]) <= j;
-      }
-      assert gain(p, sol1 + [1]) > profit2 by // from p.gains[i - 1] + profit1 > profit2, the gain of sol + gain of obj i will be bigger that previous profit
-      {
-        LastElementIs1ForGainHelper(p, sol1 + [1]);
-        assert gain(p, sol1 + [1]) == gain(p, sol1) + p.gains[i - 1];
-      }
-      assert false; 
-    } else {
-      AddingObjHasEqualGainAsOptimalSol(p, profit1, profit2, sol1, sol2, x, i, j);
-      assert gain(p, x) == gain(p, sol1 + [1]);
-    }
-  }
-}
-
 method getPartialProfits(p: Problem, profits: seq<seq<int>>, solutions : seq<seq<seq<int>>>, i: int) returns (partialProfits: seq<int>, partialSolutions: seq<seq<int>>)
   requires isValidProblem(p)
-  requires 0 < i < p.numberOfObjects + 1
+  requires 0 < i < p.n + 1
   requires i == |profits| == |solutions|
-  requires forall k :: 0 <= k < i ==> |profits[k]| == p.knapsackCapacity + 1
+  requires forall k :: 0 <= k < i ==> |profits[k]| == p.c + 1
 
-  requires forall k :: 0 <= k < i ==> |solutions[k]| == p.knapsackCapacity + 1
+  requires forall k :: 0 <= k < i ==> |solutions[k]| == p.c + 1
   requires forall k :: 0 <= k < i ==> forall q :: 0 <= q < |solutions[k]| ==> |solutions[k][q]| == k
-  requires forall k :: 0 <= k < i ==> forall q :: 0 <= q < |solutions[k]| ==> hasOnlyPermittedValues(solutions[k][q])
-  requires forall k :: 0 <= k < i ==> forall q :: 0 <= q < |solutions[k]| ==> 0 <= |solutions[k][q]| <= p.numberOfObjects
+  requires forall k :: 0 <= k < i ==> forall q :: 0 <= q < |solutions[k]| ==> hasAllowedValues(solutions[k][q])
+  requires forall k :: 0 <= k < i ==> forall q :: 0 <= q < |solutions[k]| ==> 0 <= |solutions[k][q]| <= p.n
   requires forall k :: 0 <= k < |solutions| ==> forall q :: 0 <= q < |solutions[k]| ==> 
-                    isPartialSolutionOfFirstIObjectsAndWeightJ(p, solutions[k][q], k, q)
+                    isPartialSolution(p, solutions[k][q], k, q)
 
   requires forall k :: 0 <= k < |solutions| ==> forall q :: 0 <= q < |solutions[k]| ==> 
-                    isOptimalPartialSolutionOfFirstIObjectsAndWeightJ(p, solutions[k][q], k, q) 
+                    isOptimalPartialSolution(p, solutions[k][q], k, q) 
   requires forall k :: 0 <= k < |solutions| ==> forall q :: 0 <= q < |solutions[k]| ==> 
                 gain(p, solutions[k][q]) == profits[k][q]
 
-  ensures |partialSolutions| == p.knapsackCapacity + 1
-  ensures |partialProfits| == p.knapsackCapacity + 1
-  ensures 0 <= |profits| <= p.numberOfObjects + 1 
+  ensures |partialSolutions| == p.c + 1
+  ensures |partialProfits| == p.c + 1
+  ensures 0 <= |profits| <= p.n + 1 
   ensures forall k :: 0 <= k < |partialSolutions| ==> |partialSolutions[k]| == i
-  ensures forall k :: 0 <= k < |partialSolutions| ==> hasOnlyPermittedValues(partialSolutions[k])
-  ensures forall k :: 0 <= k < |partialSolutions| ==> 0 <= |partialSolutions[k]| <= p.numberOfObjects
-  ensures forall k :: 0 <= k < |partialSolutions| ==> isPartialSolutionOfFirstIObjectsAndWeightJ(p, partialSolutions[k], i, k) 
+  ensures forall k :: 0 <= k < |partialSolutions| ==> hasAllowedValues(partialSolutions[k])
+  ensures forall k :: 0 <= k < |partialSolutions| ==> 0 <= |partialSolutions[k]| <= p.n
+  ensures forall k :: 0 <= k < |partialSolutions| ==> isPartialSolution(p, partialSolutions[k], i, k) 
 
-  ensures forall k :: 0 <= k < |partialSolutions| ==> isOptimalPartialSolutionOfFirstIObjectsAndWeightJ(p, partialSolutions[k], i, k)
+  ensures forall k :: 0 <= k < |partialSolutions| ==> isOptimalPartialSolution(p, partialSolutions[k], i, k)
   ensures forall k :: 0 <= k < |partialSolutions| ==> gain(p, partialSolutions[k]) == partialProfits[k]
 {
         partialProfits := [];
         var j := 0;
         partialSolutions := [];
 
-        while j <= p.knapsackCapacity
-          invariant 0 <= j <= p.knapsackCapacity + 1
-          invariant 0 <= |profits| <= p.numberOfObjects + 1
+        while j <= p.c
+          invariant 0 <= j <= p.c + 1
+          invariant 0 <= |profits| <= p.n + 1
           invariant |partialProfits| == j
           invariant |partialSolutions| == j
 
-          invariant forall k :: 0 <= k < |partialSolutions| ==> hasOnlyPermittedValues(partialSolutions[k])
-          invariant forall k :: 0 <= k < |partialSolutions| ==> isOptimalPartialSolutionOfFirstIObjectsAndWeightJ(p, partialSolutions[k], i, k)
+          invariant forall k :: 0 <= k < |partialSolutions| ==> hasAllowedValues(partialSolutions[k])
+          invariant forall k :: 0 <= k < |partialSolutions| ==> isOptimalPartialSolution(p, partialSolutions[k], i, k)
           invariant forall k :: 0 <= k < |partialSolutions| ==> gain(p, partialSolutions[k]) == partialProfits[k]
         {
           if j == 0 {
 
-              var currentProfit, currentSolution := caseMaximumWeightAllowedIs0(p, profits, partialProfits, partialSolutions, i, j);
+              var currentProfit, currentSolution := solveMaxCapacity0(p, i, j);
               partialProfits := partialProfits + [currentProfit];
               partialSolutions := partialSolutions + [currentSolution];
 
-              assert isOptimalPartialSolutionOfFirstIObjectsAndWeightJ(p, currentSolution, i, j);
+              assert isOptimalPartialSolution(p, currentSolution, i, j);
 
           } else {
             if p.weights[i - 1] <= j {
               if p.gains[i - 1] + profits[i - 1][j - p.weights[i - 1]] > profits[i - 1][j] {
 
-                  var currentProfit, currentSolution := caseObtainingBetterProfit(p, profits, solutions, partialProfits, partialSolutions, i, j);
+                  var currentProfit, currentSolution := solveAdd1BetterProfit(p, profits, solutions, partialProfits, partialSolutions, i, j);
                   partialProfits := partialProfits + [currentProfit];
                   partialSolutions := partialSolutions + [currentSolution];
 
-                  assert isOptimalPartialSolutionOfFirstIObjectsAndWeightJ(p, currentSolution, i, j);
+                  assert isOptimalPartialSolution(p, currentSolution, i, j);
 
               } else {
 
-                  var currentProfit, currentSolution := caseNotObtainingBetterProfit(p, profits, solutions, partialProfits, partialSolutions, i, j);
+                  var currentProfit, currentSolution := solveAdd0BetterProfit(p, profits, solutions, partialProfits, partialSolutions, i, j);
                   partialProfits := partialProfits + [currentProfit];
                   partialSolutions := partialSolutions + [currentSolution];
 
-                  assert isOptimalPartialSolutionOfFirstIObjectsAndWeightJ(p, currentSolution, i, j);
+                  assert isOptimalPartialSolution(p, currentSolution, i, j);
 
               }
             } else {
 
-                var currentProfit, currentSolution := caseObjWeightExceedsAllowedCapacity(p, profits, solutions, partialProfits, partialSolutions, i, j);
+                var currentProfit, currentSolution := SolveAdd0TooBig(p, profits, solutions, partialProfits, partialSolutions, i, j);
                 partialProfits := partialProfits + [currentProfit];
                 partialSolutions := partialSolutions + [currentSolution];
 
-                assert isOptimalPartialSolutionOfFirstIObjectsAndWeightJ(p, currentSolution, i, j);
+                assert isOptimalPartialSolution(p, currentSolution, i, j);
 
             }
           }
@@ -949,171 +928,185 @@ method getPartialProfits(p: Problem, profits: seq<seq<int>>, solutions : seq<seq
         }
 }
 
-method caseMaximumWeightAllowedIs0(p: Problem, profits: seq<seq<int>>, partialProfits: seq<int>, partialSolutions: seq<seq<int>>, i: int, j: int) returns (currentProfit: int, currentSolution: seq<int>)
+method solveMaxCapacity0(p: Problem, i: int, j: int) returns (currentProfit: int, currentSolution: Solution)
   requires isValidProblem(p)
-  requires 0 < i <= p.numberOfObjects
-  requires i == |profits|
+  requires 0 < i <= p.n
+  requires j == 0
 
-  requires |partialSolutions| == |partialProfits| == j == 0
-  requires forall k :: 0 <= k < |partialSolutions| ==> isOptimalPartialSolutionOfFirstIObjectsAndWeightJ(p, partialSolutions[k], i, k) 
-  requires forall k :: 0 <= k < |partialSolutions| ==> gain(p, partialSolutions[k]) == partialProfits[k]
-
-  ensures isOptimalPartialSolutionOfFirstIObjectsAndWeightJ(p, currentSolution, i, j)
+  ensures isOptimalPartialSolution(p, currentSolution, i, j)
   ensures currentProfit == gain(p, currentSolution)
                 
 {
     currentProfit := 0;
-    currentSolution := seq(i, w => 0);
+    currentSolution := seq(i, y => 0);
 
     assert |currentSolution| == i;
-    Weight0Lemma(p, currentSolution, |currentSolution| - 1);
+    ComputeWeightAllZeros(p, currentSolution, |currentSolution| - 1);
     assert weight(p, currentSolution) == 0 <= j;
-    assert isPartialSolutionOfFirstIObjectsAndWeightJ(p, currentSolution, i, j);
+    assert isPartialSolution(p, currentSolution, i, j);
     
-    MaximumWeightAllowedIs0(p, currentSolution, i, j);
-    Weight0ImpliesGain0(p, currentSolution, i, j);
+    OptimalSolCapacity0(p, currentSolution, i);
+    GainCapacity0(p, currentSolution, i);
     
-    assert isOptimalPartialSolutionOfFirstIObjectsAndWeightJ(p, currentSolution, i, j);
+    assert isOptimalPartialSolution(p, currentSolution, i, j);
 }
 
-method caseObtainingBetterProfit(p: Problem, profits: seq<seq<int>>, solutions: seq<seq<seq<int>>>, partialProfits: seq<int>, partialSolutions: seq<seq<int>>, i: int, j: int) returns (currentProfit: int, currentSolution: seq<int>)
+method solveAdd1BetterProfit(p: Problem, profits: seq<seq<int>>, solutions: seq<seq<seq<int>>>, partialProfits: seq<int>, partialSolutions: seq<seq<int>>, i: int, j: int) returns (currentProfit: int, currentSolution: seq<int>)
   requires isValidProblem(p)
-  requires 0 < i <= p.numberOfObjects
+  requires 0 < i <= p.n
   requires i == |profits| == |solutions|
-  requires 1 <= j <= p.knapsackCapacity
+  requires 1 <= j <= p.c
 
-  requires forall k :: 0 <= k < i ==> |profits[k]| == |solutions[k]| == p.knapsackCapacity + 1
+  requires forall k :: 0 <= k < i ==> |profits[k]| == |solutions[k]| == p.c + 1
   requires forall k :: 0 <= k < i ==> forall q :: 0 <= q < |solutions[k]| ==> |solutions[k][q]| == k
-  requires forall k :: 0 <= k < i ==> forall q :: 0 <= q < |solutions[k]| ==> hasOnlyPermittedValues(solutions[k][q])
+  requires forall k :: 0 <= k < i ==> forall q :: 0 <= q < |solutions[k]| ==> hasAllowedValues(solutions[k][q])
 
   requires forall k :: 0 <= k < |solutions| ==> forall q :: 0 <= q < |solutions[k]| ==> 
-                    isOptimalPartialSolutionOfFirstIObjectsAndWeightJ(p, solutions[k][q], k, q) 
+                    isOptimalPartialSolution(p, solutions[k][q], k, q) 
   requires forall k :: 0 <= k < |solutions| ==> forall q :: 0 <= q < |solutions[k]| ==> 
                 gain(p, solutions[k][q]) == profits[k][q]
 
   requires |partialSolutions| == |partialProfits| == j
-  requires forall k :: 0 <= k < |partialSolutions| ==> hasOnlyPermittedValues(partialSolutions[k])
-  requires forall k :: 0 <= k < |partialSolutions| ==> isOptimalPartialSolutionOfFirstIObjectsAndWeightJ(p, partialSolutions[k], i, k) 
+  requires forall k :: 0 <= k < |partialSolutions| ==> hasAllowedValues(partialSolutions[k])
+  requires forall k :: 0 <= k < |partialSolutions| ==> isOptimalPartialSolution(p, partialSolutions[k], i, k) 
   requires forall k :: 0 <= k < |partialSolutions| ==> gain(p, partialSolutions[k]) == partialProfits[k]
   
   requires p.weights[i - 1] <= j
   requires p.gains[i - 1] + profits[i - 1][j - p.weights[i - 1]] > profits[i - 1][j]
 
-  ensures isOptimalPartialSolutionOfFirstIObjectsAndWeightJ(p, currentSolution, i, j)
+  ensures isOptimalPartialSolution(p, currentSolution, i, j)
   ensures currentProfit == gain(p, currentSolution)
                 
 {
     currentProfit := p.gains[i - 1] + profits[i - 1][j - p.weights[i - 1]];
     currentSolution := solutions[i - 1][j - p.weights[i - 1]];
     
-    AddingObjectDoesNotExceedsCapacity(p, i - 1, j, currentSolution);
+    ComputeWeightFits1(p, currentSolution, i - 1, j);
     assert weight(p, currentSolution) <= j;
 
-    CaseTakingObjectLeadsToOptimal(p, profits[i - 1][j - p.weights[i - 1]], profits[i - 1][j], 
+    OptimalSolAdd1(p, profits[i - 1][j - p.weights[i - 1]], profits[i - 1][j], 
       currentSolution, solutions[i - 1][j], i, j);
 
     currentSolution := currentSolution + [1];
     assert |currentSolution| == i;
 
     assert currentSolution[..|currentSolution| - 1] == solutions[i - 1][j - p.weights[i - 1]];
-    LastElementIs1ForGainHelper(p, currentSolution);
+    GainAdd1(p, currentSolution);
     // assert gain(p, currentSolution) == gain(p, currentSolution[..|currentSolution| - 1]) + p.gains[i - 1] == currentProfit;
 
-    assert isOptimalPartialSolutionOfFirstIObjectsAndWeightJ(p, currentSolution, i, j);        
+    assert isOptimalPartialSolution(p, currentSolution, i, j);        
 }
 
-method caseNotObtainingBetterProfit(p: Problem, profits: seq<seq<int>>, solutions: seq<seq<seq<int>>>, partialProfits: seq<int>, partialSolutions: seq<seq<int>>, i: int, j: int) returns (currentProfit: int, currentSolution: seq<int>)
+method solveAdd0BetterProfit(p: Problem, profits: seq<seq<int>>, solutions: seq<seq<seq<int>>>, partialProfits: seq<int>, partialSolutions: seq<seq<int>>, i: int, j: int) returns (currentProfit: int, currentSolution: seq<int>)
   requires isValidProblem(p)
-  requires 0 < i <= p.numberOfObjects
+  requires 0 < i <= p.n
   requires i == |profits| == |solutions|
-  requires 1 <= j <= p.knapsackCapacity
+  requires 1 <= j <= p.c
 
-  requires forall k :: 0 <= k < i ==> |profits[k]| == |solutions[k]| == p.knapsackCapacity + 1
+  requires forall k :: 0 <= k < i ==> |profits[k]| == |solutions[k]| == p.c + 1
   requires forall k :: 0 <= k < i ==> forall q :: 0 <= q < |solutions[k]| ==> |solutions[k][q]| == k
-  requires forall k :: 0 <= k < i ==> forall q :: 0 <= q < |solutions[k]| ==> hasOnlyPermittedValues(solutions[k][q])
+  requires forall k :: 0 <= k < i ==> forall q :: 0 <= q < |solutions[k]| ==> hasAllowedValues(solutions[k][q])
 
   requires forall k :: 0 <= k < |solutions| ==> forall q :: 0 <= q < |solutions[k]| ==> 
-                    isOptimalPartialSolutionOfFirstIObjectsAndWeightJ(p, solutions[k][q], k, q) 
+                    isOptimalPartialSolution(p, solutions[k][q], k, q) 
   requires forall k :: 0 <= k < |solutions| ==> forall q :: 0 <= q < |solutions[k]| ==> 
                 gain(p, solutions[k][q]) == profits[k][q]
 
   requires |partialSolutions| == |partialProfits| == j
-  requires forall k :: 0 <= k < |partialSolutions| ==> hasOnlyPermittedValues(partialSolutions[k])
-  requires forall k :: 0 <= k < |partialSolutions| ==> isOptimalPartialSolutionOfFirstIObjectsAndWeightJ(p, partialSolutions[k], i, k) 
+  requires forall k :: 0 <= k < |partialSolutions| ==> hasAllowedValues(partialSolutions[k])
+  requires forall k :: 0 <= k < |partialSolutions| ==> isOptimalPartialSolution(p, partialSolutions[k], i, k) 
   requires forall k :: 0 <= k < |partialSolutions| ==> gain(p, partialSolutions[k]) == partialProfits[k]
   
   requires p.weights[i - 1] <= j
   requires p.gains[i - 1] + profits[i - 1][j - p.weights[i - 1]] <= profits[i - 1][j]
 
-  ensures isOptimalPartialSolutionOfFirstIObjectsAndWeightJ(p, currentSolution, i, j)
+  ensures isOptimalPartialSolution(p, currentSolution, i, j)
   ensures currentProfit == gain(p, currentSolution)
                 
 {
     currentProfit := profits[i - 1][j];
     currentSolution := solutions[i - 1][j];
 
-    NotAddingObjectDoesNotChangeSolWeight(p, j, currentSolution);
+    ComputeWeightFits0(p, currentSolution, j);
     assert weight(p, currentSolution) <= j;
 
-    NotTakingObjectLeadsToOptimalCase1(p, profits[i - 1][j - p.weights[i - 1]], profits[i - 1][j], 
+    OptimalSolAdd0(p, profits[i - 1][j - p.weights[i - 1]], profits[i - 1][j], 
       solutions[i - 1][j - p.weights[i - 1]], currentSolution, i, j);
 
     currentSolution := currentSolution + [0];
     assert |currentSolution| == i;
     
-    LastElementIs0ForGainHelper(p, currentSolution);
+    GainAdd0(p, currentSolution);
 
-    assert isOptimalPartialSolutionOfFirstIObjectsAndWeightJ(p, currentSolution, i, j);   
+    assert isOptimalPartialSolution(p, currentSolution, i, j);   
 }
 
-method caseObjWeightExceedsAllowedCapacity(p: Problem, profits: seq<seq<int>>, solutions: seq<seq<seq<int>>>, partialProfits: seq<int>, partialSolutions: seq<seq<int>>, i: int, j: int) returns (currentProfit: int, currentSolution: seq<int>)
-  requires isValidProblem(p)
-  requires 0 < i <= p.numberOfObjects
-  requires i == |profits| == |solutions|
-  requires 1 <= j <= p.knapsackCapacity
+ghost predicate validPartialSolutions(p: Problem, profits: seq<seq<int>>, solutions: seq<seq<seq<int>>>, partialProfits: seq<int>, partialSolutions: seq<seq<int>>, i: int, j: int) 
 
-  requires forall k :: 0 <= k < i ==> |profits[k]| == |solutions[k]| == p.knapsackCapacity + 1
+{
+  isValidProblem(p) && 1 < i <= p.n && 
+  |profits| == |solutions| == i && 
+  (forall k :: 0 <= k < i ==> |profits[k]| == |solutions[k]| == p.c + 1) && 
+  (forall k :: 0 <= k < i ==> forall q :: 0 <= q < |solutions[k]| <= p.c == |profits[k]| ==> (hasAllowedValues(solutions[k][q]) && 
+  |solutions[k][q]| == k && isOptimalPartialSolution(p, solutions[k][q], k, q) && gain(p, solutions[k][q]) == profits[k][q])) && 
+  
+  1 <= j <= p.c && 
+  |partialProfits| == |partialSolutions| == j && 
+  (forall k :: 0 <= k < |partialSolutions| ==> (hasAllowedValues(partialSolutions[k]) && 
+  isOptimalPartialSolution(p, partialSolutions[k], i, k) && gain(p, partialSolutions[k]) == partialProfits[k]))
+}
+
+method SolveAdd0TooBig(p: Problem, profits: seq<seq<int>>, solutions: seq<seq<seq<int>>>, partialProfits: seq<int>, partialSolutions: seq<seq<int>>, i: int, j: int) returns (currentProfit: int, currentSolution: seq<int>)
+  requires isValidProblem(p)
+  requires 0 < i <= p.n
+  requires i == |profits| == |solutions|
+  requires 1 <= j <= p.c
+
+  requires forall k :: 0 <= k < i ==> |profits[k]| == |solutions[k]| == p.c + 1
   requires forall k :: 0 <= k < i ==> forall q :: 0 <= q < |solutions[k]| ==> |solutions[k][q]| == k
-  requires forall k :: 0 <= k < i ==> forall q :: 0 <= q < |solutions[k]| ==> hasOnlyPermittedValues(solutions[k][q])
+  requires forall k :: 0 <= k < i ==> forall q :: 0 <= q < |solutions[k]| ==> hasAllowedValues(solutions[k][q])
 
   requires forall k :: 0 <= k < |solutions| ==> forall q :: 0 <= q < |solutions[k]| ==> 
-                    isOptimalPartialSolutionOfFirstIObjectsAndWeightJ(p, solutions[k][q], k, q) 
+                    isOptimalPartialSolution(p, solutions[k][q], k, q) 
   requires forall k :: 0 <= k < |solutions| ==> forall q :: 0 <= q < |solutions[k]| ==> 
                 gain(p, solutions[k][q]) == profits[k][q]
 
   requires |partialSolutions| == |partialProfits| == j
-  requires forall k :: 0 <= k < |partialSolutions| ==> hasOnlyPermittedValues(partialSolutions[k])
-  requires forall k :: 0 <= k < |partialSolutions| ==> isOptimalPartialSolutionOfFirstIObjectsAndWeightJ(p, partialSolutions[k], i, k) 
+  requires forall k :: 0 <= k < |partialSolutions| ==> hasAllowedValues(partialSolutions[k])
+  requires forall k :: 0 <= k < |partialSolutions| ==> isOptimalPartialSolution(p, partialSolutions[k], i, k) 
   requires forall k :: 0 <= k < |partialSolutions| ==> gain(p, partialSolutions[k]) == partialProfits[k]
+
+  // requires isOk(p, profits, solutions, partialProfits, partialSolutions, i, j)
+
   requires p.weights[i - 1] > j
 
-  ensures isOptimalPartialSolutionOfFirstIObjectsAndWeightJ(p, currentSolution, i, j)
+  ensures isOptimalPartialSolution(p, currentSolution, i, j)
   ensures currentProfit == gain(p, currentSolution)
                 
 {
     currentProfit := profits[i - 1][j];
     currentSolution := solutions[i - 1][j];
 
-    NotAddingObjectDoesNotChangeSolWeight(p, j, currentSolution);
+    ComputeWeightFits0(p, currentSolution, j);
     assert weight(p, currentSolution) <= j;
-    assert isPartialSolutionOfFirstIObjectsAndWeightJ(p, currentSolution, i - 1, j);
+    assert isPartialSolution(p, currentSolution, i - 1, j);
 
-    NotTakingObjectLeadsToOptimalCase2(p, currentSolution, i, j);
+    OptimalSolAdd0TooBig(p, currentSolution, i, j);
 
     currentSolution := currentSolution + [0];
     assert |currentSolution| == i;
-    assert isPartialSolutionOfFirstIObjectsAndWeightJ(p, currentSolution, i, j);
+    assert isPartialSolution(p, currentSolution, i, j);
     
-    LastElementIs0ForGainHelper(p, currentSolution);
+    GainAdd0(p, currentSolution);
 
-    assert isOptimalPartialSolutionOfFirstIObjectsAndWeightJ(p, currentSolution, i, j);        
+    assert isOptimalPartialSolution(p, currentSolution, i, j);        
 }
 
 method Main()
 {
-    var p: Problem := Problem(numberOfObjects := 4, knapsackCapacity := 8, 
+    var p: Problem := Problem(n := 4, c := 8, 
                                     gains := [1, 2, 5, 6], weights := [2, 3, 4, 5]);
-    var maximProfit, finalSolution := KnapsackProblem(p);
+    var maximProfit, finalSolution := Solve(p);
 
     print "\n Maximum profit is: ";
     print maximProfit;
